PhysLean/StringTheory/FTheory/SU5U1/Charges/PhenoConstrained/Basic.lean
@@ -1,0 +1,384 @@
+/-
+Copyright (c) 2025 Joseph Tooby-Smith. All rights reserved.
+Released under Apache 2.0 license as described in the file LICENSE.
+Authors: Joseph Tooby-Smith
+-/
+import PhysLean.StringTheory.FTheory.SU5U1.Potential.ChargeProfile.Irreducible.Elems
+import PhysLean.StringTheory.FTheory.SU5U1.Charges.Tree.Insert
+/-!
+
+# Pheno constrained charges
+
+We say a charge is pheno-constrained if it leads to allows proton decay or
+R-parity violating terms.
+
+We are actually intrested in the charges which are not pheno-constrained.
+
+-/
+namespace FTheory
+
+namespace SU5U1
+
+variable {I : CodimensionOneConfig}
+namespace Charges
+open PotentialTerm
+open ChargeProfile
+
+/-- A charge is pheno-constrained if it leads to the presence of any term causing proton decay
+  ` {W1, Λ, W2, K1}` or R-parity violation `{β, Λ, W2, W4, K1, K2}`. -/
+def IsPhenoConstrained (x : Charges) : Prop :=
+  IsPresent μ (toChargeProfile μ x) ∨
+  IsPresent β (toChargeProfile β x) ∨
+  IsPresent Λ (toChargeProfile Λ x) ∨
+  IsPresent W2 (toChargeProfile W2 x) ∨
+  IsPresent W4 (toChargeProfile W4 x) ∨
+  IsPresent K1 (toChargeProfile K1 x) ∨
+  IsPresent K2 (toChargeProfile K2 x) ∨
+  IsPresent W1 (toChargeProfile W1 x)
+
+instance decidableIsPhenoConstrained (x : Charges) : Decidable x.IsPhenoConstrained :=
+  inferInstanceAs (Decidable (IsPresent μ (toChargeProfile μ x) ∨
+    IsPresent β (toChargeProfile β x) ∨
+    IsPresent Λ (toChargeProfile Λ x) ∨
+    IsPresent W2 (toChargeProfile W2 x) ∨
+    IsPresent W4 (toChargeProfile W4 x) ∨
+    IsPresent K1 (toChargeProfile K1 x) ∨
+    IsPresent K2 (toChargeProfile K2 x) ∨
+    IsPresent W1 (toChargeProfile W1 x)))
+
+lemma isPhenoConstrained_of_subset {x y : Charges} (h : x ⊆ y)
+    (hx : x.IsPhenoConstrained) : y.IsPhenoConstrained := by
+  simp [IsPhenoConstrained] at *
+  rcases hx with hr | hr | hr | hr | hr | hr | hr | hr
+  all_goals
+    have h' := isPresent_of_subset (toChargeProfile_subset_of_subset _ h) hr
+    simp_all
+
+/-!
+
+## Inserting charges into trees, with pheno constraints
+
+We define two functions `phenoInsertQ10` and `phenoInsertQ5` which for a tree
+`T` respectively give all not pheno-constrained new charges obtained by inserting a
+`q10` or `q5` charge into the charges in `T`.
+
+This is related to the `insertQ10` and `insertQ5` functions, which insert a charge into a tree
+`T`, but do not check if the new charges is pheno-constrained.
+
+-/
+
+namespace Tree
+
+/-!
+
+### Inserting `q10` charges into trees
+
+-/
+
+/-- The twig obtained by taking the new, not pheno-constrained, charges obtained by inserting
+  `q10` into all leafs of a twig. This assumes that all existing charges in the twig are
+  already not pheno constrained. -/
+def Twig.phenoInsertQ10 (t : Twig) (qHd : Option ℤ) (x : ℤ) : Twig :=
+  match t with
+  | .twig Q5 leafs =>
+    if IsPresent Λ (Q5, {x}) then
+      .twig Q5 {}
+    else
+      let leafFinst := leafs.map (fun (.leaf ys) => ys)
+      let sub : Multiset (Finset ℤ) := leafFinst.filterMap (fun ys =>
+        if ¬ insert x ys ∈ leafFinst then
+          some (insert x ys)
+        else
+          none)
+      let subFilter := sub.filter (fun ys =>
+        ¬ IsPresent W1 (Q5, ys) ∧ ¬ IsPresent K1 (Q5, ys)
+        ∧ ¬ IsPresent W2 (qHd, ys))
+      .twig Q5 (subFilter.map (fun ys => .leaf ys))
+
+/-- The branch obtained by taking the new, not pheno-constrained, charges obtained by inserting
+  `q10` into all leafs of a branch. This assumes that all existing charges in the branch are
+  already not pheno constrained. -/
+def Branch.phenoInsertQ10 (b : Branch) (qHd : Option ℤ) (x : ℤ) : Branch :=
+  match b with
+  | .branch qHu twigs =>
+      if IsPresent K2 (qHd, qHu, {x}) then
+          .branch qHu {}
+      else
+        .branch qHu (twigs.map fun t => Twig.phenoInsertQ10 t qHd x)
+
+/-- The trunk obtained by taking the new, not pheno-constrained, charges obtained by inserting
+  `q10` into all leafs of a trunk. This assumes that all existing charges in the trunk are
+  already not pheno constrained. -/
+def Trunk.phenoInsertQ10 (T : Trunk) (x : ℤ) : Trunk :=
+  match T with
+  | .trunk qHd branches =>
+    .trunk qHd (branches.map fun b => Branch.phenoInsertQ10 b qHd x)
+
+/-- The tree obtained by taking the new, not pheno-constrained, charges obtained by inserting
+  `q10` into all leafs of a tree. This assumes that all existing charges in the tree are
+  already not pheno constrained. -/
+def phenoInsertQ10 (T : Tree) (x : ℤ) : Tree :=
+  match T with
+  | .root trunks =>
+    .root (trunks.map fun ts => (Trunk.phenoInsertQ10 ts x))
+
+lemma mem_insertQ10_and_not_isPresent_of_mem_phenoInsertQ10 (T : Tree) (q10 : ℤ) (C : Charges)
+    (h : C ∈ (phenoInsertQ10 T q10)) : C ∈ (T.insertQ10 q10)
+      ∧ ¬ IsPresent K2 (C.1, C.2.1, {q10})
+      ∧ ¬ IsPresent Λ (C.2.2.1, {q10})
+      ∧ ¬ IsPresent W1 (C.2.2.1, C.2.2.2) ∧ ¬ IsPresent K1 (C.2.2.1, C.2.2.2)
+      ∧ ¬ IsPresent W2 (C.1, C.2.2.2) := by
+  -- We first recover the trunk, branch, twig and leaf in T which corresponds to C.
+  simp [phenoInsertQ10, Membership.mem, mem] at h
+  obtain ⟨trunkP, trunkP_mem, hC⟩ := h
+  change trunkP ∈ (Multiset.map (fun ts => ts.phenoInsertQ10 q10) T.1) at trunkP_mem
+  simp [Multiset.mem_map] at trunkP_mem
+  -- trunkT is the trunk in T which corresponds to C. C does not live in this trunk.
+  obtain ⟨trunkT, trunkT_mem, rfl⟩ := trunkP_mem
+  simp [Trunk.mem] at hC
+  obtain ⟨C_fst, branchP, branchP_mem, hC⟩ := hC
+  simp [Trunk.phenoInsertQ10] at branchP_mem
+  -- branchT is the branch in trunkT which corresponds to C. C does not live in this branch.
+  -- C lives in branchP
+  obtain ⟨branchT, branchT_mem, branchP_eq⟩ := branchP_mem
+  by_cases hK2 : IsPresent K2 (trunkT.1, branchT.1, {q10})
+  · simp_all [Branch.phenoInsertQ10]
+    rw [← branchP_eq] at hC
+    simp [Branch.mem] at hC
+  simp_all [Branch.phenoInsertQ10]
+  match branchP with
+  | .branch qHu twigsP =>
+  simp at branchP_eq
+  obtain ⟨rfl, twigsP_eq⟩ := branchP_eq
+  simp [Branch.mem] at hC
+  obtain ⟨c_qHu_eq, twigP, twigP_mem, hC⟩ := hC
+  -- getting twigT
+  rw [← twigsP_eq] at twigP_mem
+  simp at twigP_mem
+  obtain ⟨twigT, twigT_mem, twigP_eq⟩ := twigP_mem
+  -- The condition on Λ
+  by_cases hΛ : IsPresent Λ (twigT.1, {q10})
+  · simp_all [Twig.phenoInsertQ10]
+    rw [← twigP_eq] at hC
+    simp [Twig.mem] at hC
+  simp_all [Twig.phenoInsertQ10]
+  -- Getting leafP
+  match twigP with
+  | .twig Q5 leafsP =>
+  simp at twigP_eq
+  obtain ⟨rfl, leafsP_eq⟩ := twigP_eq
+  simp [Twig.mem] at hC
+  obtain ⟨c_Q5_eq, leafP, leafP_mem, hC⟩ := hC
+  -- Getting leafT
+  rw [← leafsP_eq] at leafP_mem
+  simp at leafP_mem
+  obtain ⟨Q10P, ⟨⟨leafT, leafT_mem, h1⟩, hPresent⟩, h2⟩ := leafP_mem
+  have hQ10P : Q10P = C.2.2.2 := by
+    simp [Leaf.mem] at hC
+    rw [← hC, ← h2]
+  -- The goal
+  apply And.intro
+  · apply mem_of_parts (trunkT.insertQ10 q10) (branchT.insertQ10 q10)
+      (twigT.insertQ10 q10) (leafT.insertQ10 q10)
+    · simp [insertQ10]
+      use trunkT
+    · simp [Trunk.insertQ10]
+      use branchT
+    · simp [Branch.insertQ10]
+      use twigT
+    · simp [Twig.insertQ10]
+      use Q10P
+      constructor
+      · use leafT
+      · rw [← h1.2]
+        rfl
+    · simp_all only [Trunk.insertQ10, Branch.insertQ10, Twig.insertQ10, Leaf.insertQ10,
+        Trunk.phenoInsertQ10]
+      simp [Leaf.mem] at hC
+      rw [hC]
+      rfl
+  simp_all
+  simp [Trunk.phenoInsertQ10] at C_fst
+  simp_all
+
+lemma mem_phenoInsertQ10_of_mem_isPresent (T : Tree) (q10 : ℤ) (C : Charges)
+    (h : C ∈ (T.insertQ10 q10)) (hC : ¬ IsPresent K2 (C.1, C.2.1, {q10})
+      ∧ ¬ IsPresent Λ (C.2.2.1, {q10})
+      ∧ ¬ IsPresent W1 (C.2.2.1, C.2.2.2) ∧ ¬ IsPresent K1 (C.2.2.1, C.2.2.2)
+      ∧ ¬ IsPresent W2 (C.1, C.2.2.2)) :
+    C ∈ phenoInsertQ10 T q10 := by
+  rw [mem_iff_mem_toMultiset] at h
+  simp [toMultiset] at h
+  obtain ⟨trunkI, trunkI_mem, branchI, branchI_mem, twigI, twigI_mem,
+    leafI, leafI_mem, heq⟩ := h
+  -- obtaining trunkT
+  simp [insertQ10] at trunkI_mem
+  obtain ⟨trunkT, trunkT_mem, rfl⟩ := trunkI_mem
+  -- obtaining branchT
+  simp [Trunk.insertQ10] at branchI_mem
+  obtain ⟨branchT, branchT_mem, rfl⟩ := branchI_mem
+  -- obtaining twigT
+  simp only [Branch.insertQ10, Multiset.mem_map] at twigI_mem
+  obtain ⟨twigT, twigT_mem, rfl⟩ := twigI_mem
+  -- obtaining leafT
+  simp only [Twig.insertQ10, Multiset.mem_map, not_exists, not_and, Multiset.mem_filterMap,
+    Option.ite_none_right_eq_some, Option.some.injEq, exists_exists_and_eq_and] at leafI_mem
+  obtain ⟨Q10, ⟨leafT, leafT_mem, hQ10⟩, hPresent⟩ := leafI_mem
+  -- Properties of C
+  have hC1 : C.1 = trunkT.1 := by
+    subst heq
+    simp [Trunk.insertQ10]
+  have hC2 : C.2.1 = branchT.1 := by
+    subst heq
+    simp [Branch.insertQ10]
+  have hC21 : C.2.2.1 = twigT.1 := by
+    subst heq
+    simp [Twig.insertQ10]
+  have hC22 : C.2.2.2 = Q10 := by
+    subst heq
+    simp [Leaf.insertQ10, ← hPresent]
+  have C_eq : C = (trunkT.1, branchT.1, twigT.1, Q10) := by
+    simp [← hC1, ← hC2, ← hC21, ← hC22]
+  -- Work on the goal
+  apply mem_of_parts (trunkT.phenoInsertQ10 q10) (branchT.phenoInsertQ10
+    (trunkT.phenoInsertQ10 q10).1 q10) (twigT.phenoInsertQ10 (trunkT.phenoInsertQ10 q10).1 q10)
+    (.leaf Q10)
+  · simp [phenoInsertQ10]
+    use trunkT
+  · simp [Trunk.phenoInsertQ10]
+    use branchT
+  · simp [Branch.phenoInsertQ10]
+    rw [if_neg]
+    · simp
+      use twigT
+    · simp [Trunk.phenoInsertQ10, ← hC1, ← hC2]
+      exact hC.1
+  · simp [Twig.phenoInsertQ10]
+    rw [if_neg]
+    swap
+    · rw [← hC21]
+      exact hC.2.1
+    simp only [Multiset.mem_map, Multiset.mem_filter, Multiset.mem_filterMap,
+      Option.ite_none_right_eq_some, Option.some.injEq, exists_exists_and_eq_and, Leaf.leaf.injEq,
+      exists_eq_right]
+    constructor
+    · use leafT
+    · rw [← hC21, ← hC22]
+      simp_all [Trunk.phenoInsertQ10]
+  · subst C_eq
+    simp [Trunk.phenoInsertQ10, Branch.phenoInsertQ10]
+    rw [if_neg]
+    swap
+    · simp_all
+    simp [Twig.phenoInsertQ10]
+    rw [if_neg]
+    simp_all
+
+/-!
+
+### Inserting `q5` charges into trees
+
+-/
+
+/-- The branch obtained by taking the new, not pheno-constrained, charges obtained by inserting
+  `q5` into all leafs of a branch. This assumes that all existing charges in the branch are
+  already not pheno constrained. -/
+def Branch.phenoInsertQ5 (b : Branch) (qHd : Option ℤ) (x : ℤ) : Branch :=
+  match b with
+  | .branch qHu twigs =>
+    if IsPresent β (qHu, {x}) ∨ IsPresent W4 (qHd, qHu, {x}) then
+          .branch qHu {}
+        else
+          let insertTwigs := twigs.map (fun (.twig Q5 leafs) => Twig.twig (insert x Q5)
+            (leafs.filter (fun (.leaf Q10) => ¬ IsPresent W1 ({x}, Q10) ∧ ¬ IsPresent K1 ({x}, Q10)
+              ∧ ¬ IsPresent Λ ((insert x Q5), Q10) ∧
+              ¬ Branch.mem (.branch qHu twigs) (qHu, (insert x Q5), Q10))))
+          .branch qHu <| insertTwigs
+
+/-- The trunk obtained by taking the new, not pheno-constrained, charges obtained by inserting
+  `q5` into all leafs of a trunk. This assumes that all existing charges in the trunk are
+  already not pheno constrained. -/
+def Trunk.phenoInsertQ5 (T : Trunk) (x : ℤ) : Trunk :=
+  match T with
+  | .trunk qHd branches =>
+    .trunk qHd (branches.map fun b => b.phenoInsertQ5 qHd x)
+
+/-- The tree obtained by taking the new, not pheno-constrained, charges obtained by inserting
+  `q5` into all leafs of a tree. This assumes that all existing charges in the tree are
+  already not pheno constrained. -/
+def phenoInsertQ5 (T : Tree) (x : ℤ) : Tree :=
+  match T with
+  | .root trunks =>
+    .root (trunks.map fun ts => (Trunk.phenoInsertQ5 ts x))
+
+lemma mem_phenoInsertQ5_of_mem_isPresent (T : Tree) (q5 : ℤ) (C : Charges)
+    (h : C ∈ (T.insertQ5 q5)) (hC : ¬ IsPresent β (C.2.1, {q5})
+      ∧ ¬ IsPresent W4 (C.1, C.2.1, {q5}) ∧
+      ¬ IsPresent W1 ({q5}, C.2.2.2) ∧ ¬ IsPresent K1 ({q5}, C.2.2.2)
+      ∧ ¬ IsPresent Λ (C.2.2.1, C.2.2.2)) :
+    C ∈ phenoInsertQ5 T q5 := by
+  rw [mem_iff_mem_toMultiset] at h
+  simp [toMultiset] at h
+  obtain ⟨trunkI, trunkI_mem, branchI, branchI_mem, twigI, twigI_mem,
+    leafI, leafI_mem, heq⟩ := h
+  -- obtaining trunkT
+  simp [insertQ5] at trunkI_mem
+  obtain ⟨trunkT, trunkT_mem, rfl⟩ := trunkI_mem
+  -- obtaining branchT
+  simp [Trunk.insertQ5] at branchI_mem
+  obtain ⟨branchT, branchT_mem, rfl⟩ := branchI_mem
+  -- obtaining twigT
+  simp only [Branch.insertQ5, Multiset.mem_map] at twigI_mem
+  obtain ⟨twigT, twigT_mem, rfl⟩ := twigI_mem
+  -- obtaining leafT
+  simp [Twig.insertQ5, Multiset.mem_map, not_exists, not_and, Multiset.mem_filterMap,
+    Option.ite_none_right_eq_some, Option.some.injEq, exists_exists_and_eq_and] at leafI_mem
+  obtain ⟨leftI_mem, h_not_mem⟩ := leafI_mem
+  -- Properties of C
+  have hC1 : C.1 = trunkT.1 := by
+    subst heq
+    simp [Trunk.insertQ5]
+  have hC2 : C.2.1 = branchT.1 := by
+    subst heq
+    simp [Branch.insertQ5]
+  have hC21 : C.2.2.1 = insert q5 twigT.1 := by
+    subst heq
+    simp [Twig.insertQ5]
+  have hC22 : C.2.2.2 = leafI.1 := by
+    subst heq
+    simp [Leaf.insertQ10]
+  have C_eq : C = (trunkT.1, branchT.1, insert q5 twigT.1, leafI.1) := by
+    simp [← hC1, ← hC2, ← hC21, ← hC22]
+  -- Work on the goal
+  apply mem_of_parts (trunkT.phenoInsertQ5 q5) (branchT.phenoInsertQ5
+    (trunkT.phenoInsertQ5 q5).1 q5)
+    (Twig.twig (insert q5 twigT.1)
+        (Multiset.filter (fun (.leaf Q10) =>
+        ¬ IsPresent W1 ({q5}, Q10) ∧ ¬ IsPresent K1 ({q5}, Q10)
+          ∧ ¬ IsPresent Λ ((insert q5 twigT.1), Q10) ∧
+          ¬(Branch.branch branchT.1 branchT.2).mem (branchT.1, insert q5 twigT.1, Q10))
+          twigT.2)) (leafI)
+  · simp [phenoInsertQ5]
+    use trunkT
+  · simp [Trunk.phenoInsertQ5]
+    use branchT
+  · simp [Branch.phenoInsertQ5]
+    rw [if_neg]
+    · simp
+      use twigT
+    · simp [Trunk.phenoInsertQ5, ← hC1, ← hC2]
+      exact ⟨hC.1, hC.2.1⟩
+  · simp_all
+  · simp
+    subst C_eq
+    simp [Trunk.phenoInsertQ5, Branch.phenoInsertQ5]
+    rw [if_neg]
+    simp_all
+
+end Tree
+
+end Charges
+
+end SU5U1
+
+end FTheory
