PhysLean/StringTheory/FTheory/SU5U1/Charges/PhenoConstrained/Completeness.lean
@@ -1,0 +1,450 @@
+/-
+Copyright (c) 2025 Joseph Tooby-Smith. All rights reserved.
+Released under Apache 2.0 license as described in the file LICENSE.
+Authors: Joseph Tooby-Smith
+-/
+import PhysLean.StringTheory.FTheory.SU5U1.Potential.ChargeProfile.Irreducible.Completeness
+import PhysLean.StringTheory.FTheory.SU5U1.Charges.PhenoConstrained.Elems.IsComplete
+import PhysLean.StringTheory.FTheory.SU5U1.Charges.PhenoConstrained.Elems.PhenoConstrained
+import PhysLean.StringTheory.FTheory.SU5U1.Charges.PhenoConstrained.Elems.PhenoInsertQ10
+import PhysLean.StringTheory.FTheory.SU5U1.Charges.PhenoConstrained.Elems.PhenoInsertQ5
+/-!
+
+# Complete of `nonPhenoConstrainedCharges I`
+
+We show that the `nonPhenoConstrainedCharges I` is complete, that is,
+it contains every charge in `ofFinset I.allowedBarFiveCharges I.allowedTenCharges`
+which is not pheno-constrained, permits a top yukawa and is complete.
+
+## Method
+
+The method of our proof is the following.
+
+1. We define `completionTopYukawa` which contains all `completions` of elements
+  `irreducibleElems I topYukawa` which are not pheno-constrained. We show
+  that every charge in `ofFinset I.allowedBarFiveCharges I.allowedTenCharges`
+  which is not pheno-constrained and complete must contain an element
+  of `completionTopYukawaSame` as a subset.
+2. We show that `completionTopYukawa I` is a subset of `nonPhenoConstrainedCharges I`.
+3. We then use the fact that one can not add to any charge in `nonPhenoConstrainedCharges`
+  another `Q5` or `Q10` without remaining in `nonPhenoConstrainedCharges` or allowing
+  a pheno-constraining term to be present.
+
+This proof of completeness is more like a certification of completeness, rather
+than a constructive proof.
+
+## Key results
+
+- `not_isPhenoConstrained_iff_mem_nonPhenoConstrainedCharge` which specifies
+  the completeness of the tree of charges `nonPhenoConstrainedCharges I`.
+-/
+namespace FTheory
+
+namespace SU5U1
+
+variable {I : CodimensionOneConfig}
+
+namespace Charges
+open PotentialTerm ChargeProfile
+open CodimensionOneConfig
+
+open Tree Leaf Twig Branch Trunk
+
+set_option maxRecDepth 2000
+
+lemma nonPhenoConstrainedCharges_insertQ10_filter (I : CodimensionOneConfig) :
+    ∀ (q10 : { x // x ∈ I.allowedTenCharges }),
+      Multiset.filter (fun x => ¬x.IsPhenoConstrained)
+      ((nonPhenoConstrainedCharges I).insertQ10 ↑q10).toMultiset = ∅ := by
+  intro ⟨q10, hq10⟩
+  simp only [Multiset.empty_eq_zero]
+  rw [Multiset.filter_eq_nil]
+  intro C hC
+  intro hn
+  have hmemP : C ∈ (phenoInsertQ10 (nonPhenoConstrainedCharges I) q10) := by
+    rw [← mem_iff_mem_toMultiset] at hC
+    obtain ⟨qHd, qHu, Q5, Q10, rfl, h1⟩ := exists_of_mem_insertQ10 C q10 hC
+    apply mem_phenoInsertQ10_of_mem_isPresent
+    · exact hC
+    simp [IsPhenoConstrained, toChargeProfile] at hn
+    refine ⟨?_, ?_, ?_, ?_, ?_⟩
+    · by_contra hc
+      have hc' : IsPresent K2 (qHd, qHu, insert q10 Q10) := by
+        apply isPresent_of_subset _ hc
+        simp [Subset]
+      simp_all
+    · by_contra hc
+      have hc' : IsPresent Λ (Q5, insert q10 Q10) := by
+        apply isPresent_of_subset _ hc
+        simp [Subset]
+      simp_all
+    · by_contra hc
+      simp_all
+    · by_contra hc
+      simp_all
+    · by_contra hc
+      simp_all
+  have hemp : ((nonPhenoConstrainedCharges I).phenoInsertQ10 q10).toMultiset = ∅ := by
+    rw [Multiset.empty_eq_zero, ← Multiset.card_eq_zero]
+    have hx := nonPhenoConstrainedCharges_phenoInsertQ10_card_zero I q10 hq10
+    rw [← hx]
+    rw [Tree.card_eq_toMultiset_card]
+  rw [mem_iff_mem_toMultiset] at hmemP
+  simp_all
+
+lemma nonPhenoConstrainedCharges_insertQ5_filter (I : CodimensionOneConfig) :
+    ∀ (q5 : { x // x ∈ I.allowedBarFiveCharges }),
+      Multiset.filter (fun x => ¬x.IsPhenoConstrained)
+      ((nonPhenoConstrainedCharges I).insertQ5 ↑q5).toMultiset = ∅ := by
+  intro ⟨q5, hq5⟩
+  simp only [Multiset.empty_eq_zero]
+  rw [Multiset.filter_eq_nil]
+  intro C hC
+  intro hn
+  have hmemP : C ∈ (phenoInsertQ5 (nonPhenoConstrainedCharges I) q5) := by
+    rw [← mem_iff_mem_toMultiset] at hC
+    obtain ⟨qHd, qHu, Q5, Q10, rfl, h1⟩ := exists_of_mem_insertQ5 C q5 hC
+    apply mem_phenoInsertQ5_of_mem_isPresent
+    · exact hC
+    simp [IsPhenoConstrained, toChargeProfile] at hn
+    refine ⟨?_, ?_, ?_, ?_, ?_⟩
+    · by_contra hc
+      have hc' : IsPresent β (qHu, insert q5 Q5) := by
+        apply isPresent_of_subset _ hc
+        simp [Subset]
+      simp_all
+    · by_contra hc
+      have hc' : IsPresent W4 (qHd, qHu, insert q5 Q5) := by
+        apply isPresent_of_subset _ hc
+        simp [Subset]
+      simp_all
+    · by_contra hc
+      have hc' : IsPresent W1 (insert q5 Q5, Q10) := by
+        apply isPresent_of_subset _ hc
+        simp [Subset]
+      simp_all
+    · by_contra hc
+      have hc' : IsPresent K1 (insert q5 Q5, Q10) := by
+        apply isPresent_of_subset _ hc
+        simp [Subset]
+      simp_all
+    · by_contra hc
+      simp_all
+  have hemp : ((nonPhenoConstrainedCharges I).phenoInsertQ5 q5).toMultiset = ∅ := by
+    rw [Multiset.empty_eq_zero, ← Multiset.card_eq_zero]
+    have hx := nonPhenoConstrainedCharges_phenoInsertQ5_card_zero I q5 hq5
+    rw [← hx]
+    rw [Tree.card_eq_toMultiset_card]
+  rw [mem_iff_mem_toMultiset] at hmemP
+  simp_all
+
+/--
+The tree of charges which contains all `completions` of elements `irreducibleElems .same topYukawa`
+which are not pheno-constrained.
+
+This can be constructed via
+
+Tree.fromMultiset ((((irreducibleElems same topYukawa).map (fromChargeProfile topYukawa)).bind
+    (completions same.allowedBarFiveCharges same.allowedTenCharges)).dedup.filter
+    (fun x => ¬ IsPhenoConstrained x))
+-/
+def completionTopYukawa (I : CodimensionOneConfig) : Tree :=
+  match I with
+  | same => root {trunk (some (-3)) {branch (some 3) {twig {-1} {leaf {-2, -1}}, twig {0}
+        {leaf {-2, -1}}, twig {2} {leaf {-2, -1}}},
+      branch (some (-2)) {twig {0} {leaf {-2, -1}}, twig {1} {leaf {-3, 0}},
+        twig {2} {leaf {-2, -1}, leaf {-3, 0}}},
+      branch (some (-1)) {twig {0} {leaf {-2, -1}}, twig {-2} {leaf {-3, 0}},
+        twig {2} {leaf {-2, -1}, leaf {-3, 0}}},
+      branch (some 0) {twig {-2} {leaf {-3, 0}},
+      twig {-1} {leaf {-2, -1}, leaf {-3, 0}},
+      twig {1} {leaf {-3, 0}},
+      twig {2} {leaf {-2, -1}, leaf {-3, 0}}},
+      branch (some 1) {twig {0} {leaf {-2, -1}},
+      twig {-2} {leaf {-3, 0}},
+      twig {-1} {leaf {-2, -1}, leaf {-3, 0}},
+      twig {2} {leaf {-2, -1}, leaf {-3, 0}}},
+      branch (some 2) {twig {0} {leaf {-2, -1}}, twig {-2} {leaf {-3, 0}},
+        twig {-1} {leaf {-2, -1}, leaf {-3, 0}}, twig {1} {leaf {-3, 0}}}},
+    trunk (some (-2)) {branch (some 1) {twig {0} {leaf {-1}},
+      twig {2} {leaf {-1}},
+      twig {-3} {leaf {-1}, leaf {-2, 0}},
+      twig {-1} {leaf {-1}, leaf {-2, 0}},
+      twig {3} {leaf {-2, 0}}},
+      branch (some (-3)) {twig {1} {leaf {-1}},
+      twig {2} {leaf {-1}},
+      twig {-1} {leaf {-1}, leaf {-2, 0}, leaf {-3, 1}},
+      twig {0} {leaf {-1}, leaf {-3, 1}},
+      twig {3} {leaf {-2, 0}, leaf {-3, 1}}},
+      branch (some (-1)) {twig {1} {leaf {-1}}, twig {2} {leaf {-1}},
+        twig {-3} {leaf {-1}, leaf {-2, 0}}, twig {3} {leaf {-2, 0}, leaf {-3, 1}}},
+      branch (some 0) {twig {1} {leaf {-1}},
+      twig {-3} {leaf {-1}, leaf {-2, 0}},
+      twig {-1} {leaf {-1}, leaf {-2, 0}, leaf {-3, 1}},
+      twig {3} {leaf {-2, 0}, leaf {-3, 1}}},
+      branch (some 2) {twig {-3} {leaf {-1}},
+      twig {1} {leaf {-1}},
+      twig {-1} {leaf {-1}, leaf {-3, 1}},
+      twig {0} {leaf {-1}, leaf {-3, 1}},
+      twig {3} {leaf {-3, 1}}},
+      branch (some 3) {twig {-3} {leaf {-2, 0}}, twig {-1} {leaf {-2, 0}, leaf {-3, 1}},
+        twig {0} {leaf {-3, 1}}}},
+    trunk (some (-1)) {branch (some 0) {twig {-3} {leaf {-1, 0}}},
+      branch (some 3) {twig {-3} {leaf {-1, 0}}},
+      branch (some (-3)) {twig {-2} {leaf {-2, 1}}},
+      branch (some 1) {twig {-2} {leaf {-2, 1}}},
+      branch (some 2) {twig {-2} {leaf {-2, 1}}}},
+    trunk (some 0) {branch (some (-3)) {twig {3} {leaf {-2, 2}}},
+      branch (some 3) {twig {-3} {leaf {-2, 2}}},
+      branch (some (-2)) {twig {-1} {leaf {-3, 3}}, twig {1} {leaf {-3, 3}},
+        twig {2} {leaf {-3, 3}}},
+      branch (some (-1)) {twig {-3} {leaf {-2, 2}}, twig {3} {leaf {-2, 2}},
+        twig {1} {leaf {-3, 3}}, twig {2} {leaf {-3, 3}}},
+      branch (some 1) {twig {-3} {leaf {-2, 2}}, twig {3} {leaf {-2, 2}},
+        twig {-2} {leaf {-3, 3}}, twig {-1} {leaf {-3, 3}}},
+      branch (some 2) {twig {-2} {leaf {-3, 3}}, twig {-1} {leaf {-3, 3}},
+        twig {1} {leaf {-3, 3}}}},
+    trunk (some 1) {branch (some (-3)) {twig {3} {leaf {0, 1}}},
+      branch (some 0) {twig {3} {leaf {0, 1}}},
+      branch (some (-2)) {twig {2} {leaf {-1, 2}}},
+      branch (some (-1)) {twig {2} {leaf {-1, 2}}},
+      branch (some 3) {twig {2} {leaf {-1, 2}}}},
+    trunk (some 2) {branch (some (-1)) {twig {-2} {leaf {1}},
+      twig {0} {leaf {1}},
+      twig {-3} {leaf {0, 2}},
+      twig {1} {leaf {1}, leaf {0, 2}},
+      twig {3} {leaf {1}, leaf {0, 2}}},
+      branch (some (-3)) {twig {3} {leaf {0, 2}}, twig {0} {leaf {-1, 3}},
+        twig {1} {leaf {0, 2}, leaf {-1, 3}}},
+      branch (some (-2)) {twig {-1} {leaf {1}},
+      twig {3} {leaf {1}},
+      twig {-3} {leaf {-1, 3}},
+      twig {0} {leaf {1}, leaf {-1, 3}},
+      twig {1} {leaf {1}, leaf {-1, 3}}},
+      branch (some 0) {twig {-1} {leaf {1}},
+      twig {3} {leaf {1}, leaf {0, 2}},
+      twig {-3} {leaf {0, 2}, leaf {-1, 3}},
+      twig {1} {leaf {1}, leaf {0, 2}, leaf {-1, 3}}},
+      branch (some 1) {twig {-2} {leaf {1}}, twig {-1} {leaf {1}},
+        twig {3} {leaf {1}, leaf {0, 2}}, twig {-3} {leaf {0, 2}, leaf {-1, 3}}},
+      branch (some 3) {twig {-2} {leaf {1}},
+      twig {-1} {leaf {1}},
+      twig {-3} {leaf {0, 2}, leaf {-1, 3}},
+      twig {0} {leaf {1}, leaf {-1, 3}},
+      twig {1} {leaf {1}, leaf {0, 2}, leaf {-1, 3}}}},
+    trunk (some 3) {branch (some (-3)) {twig {-2} {leaf {1, 2}}, twig {0} {leaf {1, 2}},
+        twig {1} {leaf {1, 2}}},
+      branch (some (-2)) {twig {0} {leaf {1, 2}}, twig {-1} {leaf {0, 3}},
+        twig {1} {leaf {1, 2}, leaf {0, 3}}, twig {2} {leaf {0, 3}}},
+      branch (some (-1)) {twig {0} {leaf {1, 2}},
+      twig {-2} {leaf {1, 2}, leaf {0, 3}},
+      twig {1} {leaf {1, 2}, leaf {0, 3}},
+      twig {2} {leaf {0, 3}}},
+      branch (some 0) {twig {-2} {leaf {1, 2}, leaf {0, 3}},
+      twig {-1} {leaf {0, 3}},
+      twig {1} {leaf {1, 2}, leaf {0, 3}},
+      twig {2} {leaf {0, 3}}},
+      branch (some 1) {twig {0} {leaf {1, 2}}, twig {-2} {leaf {1, 2}, leaf {0, 3}},
+        twig {2} {leaf {0, 3}}},
+      branch (some 2) {twig {0} {leaf {1, 2}}, twig {-2} {leaf {1, 2}, leaf {0, 3}},
+        twig {-1} {leaf {0, 3}}}}}
+  | nearestNeighbor => root {trunk (some (-14)) {branch (some (-9)) {twig {1} {leaf {-7}},
+        twig {6} {leaf {-7}}, twig {11} {leaf {-7}, leaf {-12, -2}}},
+      branch (some (-4)) {twig {1} {leaf {-7}}, twig {-9} {leaf {-7}, leaf {-12, -2}},
+        twig {11} {leaf {-7}, leaf {-12, -2}}},
+      branch (some 1) {twig {-4} {leaf {-7}},
+      twig {6} {leaf {-7}},
+      twig {-9} {leaf {-7}, leaf {-12, -2}},
+      twig {11} {leaf {-7}, leaf {-12, -2}}},
+      branch (some 6) {twig {-4} {leaf {-7}},
+      twig {1} {leaf {-7}},
+      twig {-9} {leaf {-7}, leaf {-12, -2}},
+      twig {11} {leaf {-7}, leaf {-12, -2}}},
+      branch (some 11) {twig {-4} {leaf {-7}}, twig {1} {leaf {-7}}, twig {6} {leaf {-7}},
+        twig {-9} {leaf {-7}, leaf {-12, -2}}}},
+    trunk (some (-4)) {branch (some (-14)) {twig {-9} {leaf {-2}}, twig {11} {leaf {-2}}},
+      branch (some (-9)) {twig {11} {leaf {-2}}},
+      branch (some 1) {twig {-14} {leaf {-2}}, twig {-9} {leaf {-2}}, twig {11} {leaf {-2}}},
+      branch (some 11) {twig {-14} {leaf {-2}}, twig {-9} {leaf {-2}}}},
+    trunk (some 1) {branch (some (-14)) {twig {11} {leaf {-7, 8}}},
+      branch (some (-4)) {twig {11} {leaf {-7, 8}}},
+      branch (some (-9)) {twig {-4} {leaf {-12, 13}}},
+      branch (some 6) {twig {-9} {leaf {-12, 13}}, twig {-4} {leaf {-12, 13}}}},
+    trunk (some 6) {branch (some 1) {twig {-14} {leaf {3}}, twig {11} {leaf {3}}},
+      branch (some (-14)) {twig {1} {leaf {3}},
+      twig {-9} {leaf {-7, 13}},
+      twig {-4} {leaf {3}, leaf {-7, 13}},
+      twig {11} {leaf {3}, leaf {-7, 13}}},
+      branch (some (-9)) {twig {-4} {leaf {-7, 13}}, twig {11} {leaf {-7, 13}}},
+      branch (some (-4)) {twig {1} {leaf {3}}, twig {-9} {leaf {-7, 13}},
+        twig {11} {leaf {3}, leaf {-7, 13}}},
+      branch (some 11) {twig {-14} {leaf {3}}, twig {1} {leaf {3}}, twig {-9} {leaf {-7, 13}},
+        twig {-4} {leaf {3}, leaf {-7, 13}}}},
+    trunk (some 11) {branch (some (-9)) {twig {1} {leaf {3, 8}}},
+      branch (some (-4)) {twig {1} {leaf {3, 8}}, twig {-14} {leaf {-2, 13}}},
+      branch (some 1) {twig {-14} {leaf {-2, 13}}},
+      branch (some 6) {twig {-14} {leaf {-2, 13}}}}}
+  | nextToNearestNeighbor => root {trunk (some (-13)) {
+      branch (some (-8)) {twig {7} {leaf {-9, -4}}},
+      branch (some 2) {twig {-3} {leaf {-9, -4}}, twig {7} {leaf {-9, -4}}},
+      branch (some 7) {twig {-3} {leaf {-9, -4}}},
+      branch (some 12) {twig {-3} {leaf {-9, -4}}, twig {7} {leaf {-9, -4}}}},
+    trunk (some (-8)) {branch (some 7) {twig {-13} {leaf {-4}}, twig {-3} {leaf {-4}}},
+      branch (some (-13)) {twig {-3} {leaf {-4}}, twig {7} {leaf {-4}}, twig {12} {leaf {-9, 1}}},
+      branch (some (-3)) {twig {7} {leaf {-4}}, twig {-13} {leaf {-4}, leaf {-9, 1}},
+        twig {12} {leaf {-9, 1}}},
+      branch (some 2) {twig {-3} {leaf {-4}}, twig {7} {leaf {-4}},
+        twig {-13} {leaf {-4}, leaf {-9, 1}}},
+      branch (some 12) {twig {-13} {leaf {-9, 1}}}},
+    trunk (some 2) {branch (some (-13)) {twig {-8} {leaf {1}}, twig {7} {leaf {1}},
+        twig {12} {leaf {1}}},
+      branch (some 7) {twig {-13} {leaf {1}}, twig {-8} {leaf {1}}},
+      branch (some (-8)) {twig {-13} {leaf {1}}, twig {7} {leaf {1}}, twig {-3} {leaf {-9, 11}},
+        twig {12} {leaf {1}, leaf {-9, 11}}},
+      branch (some (-3)) {twig {12} {leaf {-9, 11}}},
+      branch (some 12) {twig {-13} {leaf {1}}, twig {7} {leaf {1}},
+        twig {-8} {leaf {1}, leaf {-9, 11}}, twig {-3} {leaf {-9, 11}}}},
+    trunk (some 7) {branch (some (-8)) {twig {-13} {leaf {-4, 11}}},
+      branch (some 2) {twig {-13} {leaf {-4, 11}}},
+      branch (some 12) {twig {-13} {leaf {-4, 11}}}},
+    trunk (some 12) {branch (some (-13)) {twig {-8} {leaf {6}},
+        twig {2} {leaf {6}}, twig {7} {leaf {6}}},
+      branch (some (-8)) {twig {-13} {leaf {6}}, twig {2} {leaf {6}},
+        twig {7} {leaf {6}, leaf {1, 11}}},
+      branch (some (-3)) {twig {-13} {leaf {6}}, twig {2} {leaf {6}},
+        twig {-8} {leaf {6}, leaf {1, 11}}, twig {7} {leaf {6}, leaf {1, 11}}},
+      branch (some 2) {twig {-13} {leaf {6}}, twig {7} {leaf {6}, leaf {1, 11}}},
+      branch (some 7) {twig {-13} {leaf {6}}, twig {-8} {leaf {6}, leaf {1, 11}}}}}
+
+lemma completionTopYukawa_complete_of_same :
+    ∀ x ∈ (irreducibleElems .same topYukawa).map (fromChargeProfile topYukawa),
+    ¬ x.IsPhenoConstrained →
+    ∀ y ∈ completions same.allowedBarFiveCharges same.allowedTenCharges x, ¬ y.IsPhenoConstrained
+    → y ∈ completionTopYukawa .same := by
+  decide
+
+lemma completionTopYukawa_complete_of_nearestNeighbor :
+    ∀ x ∈ (irreducibleElems .nearestNeighbor topYukawa).map
+    (fromChargeProfile topYukawa), ¬ x.IsPhenoConstrained →
+    ∀ y ∈ completions nearestNeighbor.allowedBarFiveCharges nearestNeighbor.allowedTenCharges x,
+    ¬ y.IsPhenoConstrained
+    → y ∈ completionTopYukawa .nearestNeighbor := by
+  decide
+
+lemma completionTopYukawa_complete_of_nextToNearestNeighbor :
+    ∀ x ∈ (irreducibleElems .nextToNearestNeighbor topYukawa).map
+    (fromChargeProfile topYukawa), ¬ x.IsPhenoConstrained →
+    ∀ y ∈ completions nextToNearestNeighbor.allowedBarFiveCharges
+      nextToNearestNeighbor.allowedTenCharges x, ¬ y.IsPhenoConstrained
+    → y ∈ completionTopYukawa .nextToNearestNeighbor := by
+  decide
+
+lemma completionTopYukawa_complete {I : CodimensionOneConfig} (x : Charges)
+    (hx : x ∈ (irreducibleElems I topYukawa).map (fromChargeProfile topYukawa))
+    (hPheno : ¬ x.IsPhenoConstrained) :
+    ∀ y ∈ completions I.allowedBarFiveCharges I.allowedTenCharges x, ¬ y.IsPhenoConstrained
+    → y ∈ completionTopYukawa I := by
+  cases I
+  case same => exact completionTopYukawa_complete_of_same x hx hPheno
+  case nearestNeighbor => exact completionTopYukawa_complete_of_nearestNeighbor x hx hPheno
+  case nextToNearestNeighbor => exact
+    completionTopYukawa_complete_of_nextToNearestNeighbor x hx hPheno
+
+set_option maxRecDepth 2000 in
+lemma exists_subset_completionTopYukawa_of_not_isPhenoConstrained {x : Charges}
+    (hx : ¬ x.IsPhenoConstrained)
+    (htopYukawa : IsPresent topYukawa (toChargeProfile topYukawa x))
+    (hsub : x ∈ ofFinset I.allowedBarFiveCharges I.allowedTenCharges)
+    (hcomplete : IsComplete x) : ∃ y ∈ completionTopYukawa I, y ⊆ x := by
+  have hIrreducible :
+        ∃ y ∈ (irreducibleElems I topYukawa).map (fromChargeProfile topYukawa), y ⊆ x := by
+      rw [isPresent_iff_subest_isIrreducible] at htopYukawa
+      obtain ⟨y, hPower, hIrre⟩ := htopYukawa
+      use fromChargeProfile topYukawa y
+      constructor
+      · simp only [Multiset.mem_map]
+        use y
+        simp only [and_true]
+        rw [← isIrreducible_iff_mem_irreducibleElems]
+        · exact hIrre
+        · rw [finsetOfCodimensionOneConfig]
+          simp at hPower
+          apply ChargeProfile.mem_ofFinset_of_subset _ _ hPower
+          apply toChargeProfile_mem_ofFinset_of_mem_ofFinset topYukawa I.allowedBarFiveCharges
+            I.allowedTenCharges
+          exact hsub
+      · simp at hPower
+        have hx : fromChargeProfile topYukawa y ⊆
+            fromChargeProfile topYukawa (toChargeProfile topYukawa x) := by
+          simpa using hPower
+        apply subset_trans hx
+        exact toChargeProfile_fromChargeProfile_subset
+  obtain ⟨y, hyMem, hysubsetx⟩ := hIrreducible
+  obtain ⟨z, hz1, hz2⟩ := exist_completions_subset_of_complete
+    I.allowedBarFiveCharges I.allowedTenCharges y x hysubsetx hsub hcomplete
+  use z
+  constructor
+  · refine completionTopYukawa_complete y hyMem ?_ z hz1 ?_
+    · by_contra hn
+      have h' := isPhenoConstrained_of_subset hysubsetx hn
+      simp_all
+    · by_contra hn
+      have h' := isPhenoConstrained_of_subset hz2 hn
+      simp_all
+  · simp_all
+
+set_option maxRecDepth 2000 in
+lemma completionTopYukawa_subset_nonPhenoConstrainedCharges :
+    ∀ x ∈ (completionTopYukawa I).toMultiset, x ∈ nonPhenoConstrainedCharges I := by
+  decide +revert
+
+set_option maxRecDepth 2000 in
+lemma not_isPhenoConstrained_mem_nonPhenoConstrainedCharges {x : Charges}
+    (hx : ¬ x.IsPhenoConstrained)
+    (hsub : x ∈ ofFinset I.allowedBarFiveCharges I.allowedTenCharges)
+    (hcomplete : IsComplete x) :
+    x ∉ nonPhenoConstrainedCharges I → ¬ (¬ IsPhenoConstrained x ∧
+      IsPresent topYukawa (toChargeProfile topYukawa x)) := by
+  by_cases hn : ¬ (IsPresent topYukawa (toChargeProfile topYukawa x))
+  · simp [hn]
+  simp only [not_and, hn, imp_false]
+  simp at hn
+  obtain ⟨y, y_mem, hyx⟩ :=
+    exists_subset_completionTopYukawa_of_not_isPhenoConstrained hx hn hsub hcomplete
+  refine subset_insert_filter_card_zero (nonPhenoConstrainedCharges I)
+    I.allowedBarFiveCharges I.allowedTenCharges (fun x => ¬x.IsPhenoConstrained)
+    ?_ ?_ y ?_ x hyx hsub ?_ ?_
+  · intro x y hxy
+    simp only [Decidable.not_not]
+    exact fun a => isPhenoConstrained_of_subset hxy a
+  · intro x
+    rw [mem_iff_mem_toMultiset]
+    exact fun a => isComplete_of_mem_nonPhenoConstrainedCharge I x a
+  · apply completionTopYukawa_subset_nonPhenoConstrainedCharges
+    rw [mem_iff_mem_toMultiset] at y_mem
+    exact y_mem
+  · exact nonPhenoConstrainedCharges_insertQ10_filter I
+  · exact nonPhenoConstrainedCharges_insertQ5_filter I
+
+lemma not_isPhenoConstrained_iff_mem_nonPhenoConstrainedCharge {x : Charges}
+    (hsub : x ∈ ofFinset I.allowedBarFiveCharges I.allowedTenCharges) :
+    IsPresent topYukawa (toChargeProfile topYukawa x) ∧
+    ¬ IsPhenoConstrained x ∧ IsComplete x ↔
+    x ∈ nonPhenoConstrainedCharges I := by
+  constructor
+  · intro ⟨hTop, hPheno, hComplete⟩
+    by_contra hn
+    apply not_isPhenoConstrained_mem_nonPhenoConstrainedCharges hPheno hsub hComplete hn
+    simp_all
+  · intro h
+    rw [mem_iff_mem_toMultiset] at h
+    refine ⟨?_, ?_, ?_⟩
+    · exact isPresent_topYukawa_of_mem_nonPhenoConstrainedCharges I x h
+    · exact not_isPhenoConstrained_of_mem_nonPhenoConstrainedCharges I x h
+    · exact isComplete_of_mem_nonPhenoConstrainedCharge I x h
+
+end Charges
+
+end SU5U1
+
+end FTheory
