PhysLean/StringTheory/FTheory/SU5U1/Charges/PhenoConstrained/Elems/Card.lean
@@ -1,0 +1,38 @@
+/-
+Copyright (c) 2025 Joseph Tooby-Smith. All rights reserved.
+Released under Apache 2.0 license as described in the file LICENSE.
+Authors: Joseph Tooby-Smith
+-/
+import PhysLean.StringTheory.FTheory.SU5U1.Charges.PhenoConstrained.Elems.Basic
+/-!
+
+# Cardinality of nonPhenoConstrainedCharges
+
+-/
+namespace FTheory
+
+namespace SU5U1
+
+variable {I : CodimensionOneConfig}
+namespace Charges
+open PotentialTerm
+open ChargeProfile
+open CodimensionOneConfig
+open Tree Leaf Twig Branch Trunk
+
+lemma nonPhenoConstrainedCharges_same_card : (nonPhenoConstrainedCharges same).card = 480 := by
+  rfl
+
+lemma nonPhenoConstrainedCharges_nearestNeighbor_card :
+    (nonPhenoConstrainedCharges nearestNeighbor).card = 169 := by
+  rfl
+
+lemma nonPhenoConstrainedCharges_nextToNearestNeighbor_card :
+    (nonPhenoConstrainedCharges nextToNearestNeighbor).card = 117 := by
+  rfl
+
+end Charges
+
+end SU5U1
+
+end FTheory
