PhysLean/StringTheory/FTheory/SU5U1/Charges/PhenoConstrained/Elems/IsComplete.lean
@@ -1,0 +1,52 @@
+/-
+Copyright (c) 2025 Joseph Tooby-Smith. All rights reserved.
+Released under Apache 2.0 license as described in the file LICENSE.
+Authors: Joseph Tooby-Smith
+-/
+import PhysLean.StringTheory.FTheory.SU5U1.Charges.PhenoConstrained.Elems.Basic
+/-!
+
+# IsComplete of nonPhenoConstrainedCharges
+
+We prove that each charge in the trees `nonPhenoConstrainedCharges I`,
+is complete.
+
+-/
+namespace FTheory
+
+namespace SU5U1
+
+variable {I : CodimensionOneConfig}
+namespace Charges
+open PotentialTerm
+open ChargeProfile
+open CodimensionOneConfig
+open Tree Leaf Twig Branch Trunk
+
+set_option maxRecDepth 2000 in
+lemma isComplete_of_mem_nonPhenoConstrainedCharge_same :
+    ∀ x ∈ (nonPhenoConstrainedCharges same).toMultiset, x.IsComplete := by
+  decide
+
+set_option maxRecDepth 2000 in
+lemma isComplete_of_mem_nonPhenoConstrainedCharge_nearestNeighbor :
+    ∀ x ∈ (nonPhenoConstrainedCharges nearestNeighbor).toMultiset, x.IsComplete := by
+  decide
+
+set_option maxRecDepth 2000 in
+lemma isComplete_of_mem_nonPhenoConstrainedCharge_nextToNearestNeighbor :
+    ∀ x ∈ (nonPhenoConstrainedCharges nextToNearestNeighbor).toMultiset, x.IsComplete := by
+  decide
+
+lemma isComplete_of_mem_nonPhenoConstrainedCharge (I : CodimensionOneConfig) :
+    ∀ x ∈ (nonPhenoConstrainedCharges I).toMultiset, x.IsComplete :=
+  match I with
+  | same => isComplete_of_mem_nonPhenoConstrainedCharge_same
+  | nearestNeighbor => isComplete_of_mem_nonPhenoConstrainedCharge_nearestNeighbor
+  | nextToNearestNeighbor => isComplete_of_mem_nonPhenoConstrainedCharge_nextToNearestNeighbor
+
+end Charges
+
+end SU5U1
+
+end FTheory
