PhysLean/StringTheory/FTheory/SU5U1/Charges/PhenoConstrained/Elems/PhenoConstrained.lean
@@ -1,0 +1,93 @@
+/-
+Copyright (c) 2025 Joseph Tooby-Smith. All rights reserved.
+Released under Apache 2.0 license as described in the file LICENSE.
+Authors: Joseph Tooby-Smith
+-/
+import PhysLean.StringTheory.FTheory.SU5U1.Charges.PhenoConstrained.Elems.Basic
+/-!
+
+# Pheno constraints of nonPhenoConstrainedCharges
+
+We prove that each charge in the trees `nonPhenoConstrainedCharges I`,
+is not pheno-constrained and permits a top Yukawa.
+
+-/
+namespace FTheory
+
+namespace SU5U1
+
+variable {I : CodimensionOneConfig}
+namespace Charges
+open PotentialTerm
+open ChargeProfile
+open CodimensionOneConfig
+open Tree Leaf Twig Branch Trunk
+
+/-!
+
+### Each change is not pheno-constrained
+
+-/
+
+set_option maxRecDepth 2000 in
+lemma not_isPhenoConstrained_of_mem_nonPhenoConstrainedCharges_same :
+    ∀ x ∈ (nonPhenoConstrainedCharges same).toMultiset, ¬ x.IsPhenoConstrained := by
+  decide
+
+set_option maxRecDepth 2000 in
+lemma not_isPhenoConstrained_of_mem_nonPhenoConstrainedCharges_nearestNeighbor :
+    ∀ x ∈ (nonPhenoConstrainedCharges nearestNeighbor).toMultiset, ¬ x.IsPhenoConstrained := by
+  decide
+
+set_option maxRecDepth 2000 in
+lemma not_isPhenoConstrained_of_mem_nonPhenoConstrainedCharges_nextToNearestNeighbor :
+    ∀ x ∈ (nonPhenoConstrainedCharges nextToNearestNeighbor).toMultiset,
+      ¬ x.IsPhenoConstrained := by
+  decide
+
+lemma not_isPhenoConstrained_of_mem_nonPhenoConstrainedCharges (I : CodimensionOneConfig) :
+    ∀ x ∈ (nonPhenoConstrainedCharges I).toMultiset, ¬ x.IsPhenoConstrained :=
+  match I with
+  | same => not_isPhenoConstrained_of_mem_nonPhenoConstrainedCharges_same
+  | nearestNeighbor => not_isPhenoConstrained_of_mem_nonPhenoConstrainedCharges_nearestNeighbor
+  | nextToNearestNeighbor =>
+    not_isPhenoConstrained_of_mem_nonPhenoConstrainedCharges_nextToNearestNeighbor
+
+/-!
+
+### Each change has a top Yukawa coupling
+
+-/
+
+set_option maxRecDepth 2000 in
+lemma isPresent_topYukawa_of_mem_nonPhenoConstrainedCharges_same :
+    ∀ x ∈ (nonPhenoConstrainedCharges same).toMultiset,
+      IsPresent topYukawa (toChargeProfile topYukawa x) := by
+  decide
+
+set_option maxRecDepth 2000 in
+lemma isPresent_topYukawa_of_mem_nonPhenoConstrainedCharges_nearestNeighbor :
+    ∀ x ∈ (nonPhenoConstrainedCharges nearestNeighbor).toMultiset,
+      IsPresent topYukawa (toChargeProfile topYukawa x) := by
+  decide
+
+set_option maxRecDepth 2000 in
+lemma isPresent_topYukawa_of_mem_nonPhenoConstrainedCharges_nextToNearestNeighbor :
+    ∀ x ∈ (nonPhenoConstrainedCharges nextToNearestNeighbor).toMultiset,
+      IsPresent topYukawa (toChargeProfile topYukawa x) := by
+  decide
+
+lemma isPresent_topYukawa_of_mem_nonPhenoConstrainedCharges (I : CodimensionOneConfig) :
+    ∀ x ∈ (nonPhenoConstrainedCharges I).toMultiset,
+      IsPresent topYukawa (toChargeProfile topYukawa x) :=
+  match I with
+  | same => isPresent_topYukawa_of_mem_nonPhenoConstrainedCharges_same
+  | nearestNeighbor => isPresent_topYukawa_of_mem_nonPhenoConstrainedCharges_nearestNeighbor
+  | nextToNearestNeighbor =>
+    isPresent_topYukawa_of_mem_nonPhenoConstrainedCharges_nextToNearestNeighbor
+
+end Charges
+
+end SU5U1
+
+end FTheory
