PhysLean/StringTheory/FTheory/SU5U1/Charges/PhenoConstrained/Elems/PhenoInsertQ5.lean
@@ -1,0 +1,62 @@
+/-
+Copyright (c) 2025 Joseph Tooby-Smith. All rights reserved.
+Released under Apache 2.0 license as described in the file LICENSE.
+Authors: Joseph Tooby-Smith
+-/
+import PhysLean.StringTheory.FTheory.SU5U1.Charges.PhenoConstrained.Elems.Basic
+/-!
+
+# PhenoInsert of nonPhenoConstrainedCharges
+
+We prove show that the phenoInsertQ5
+of `nonPhenoConstrainedCharges I` is empty. This result is used
+in the completeness proof.
+
+-/
+namespace FTheory
+
+namespace SU5U1
+
+variable {I : CodimensionOneConfig}
+namespace Charges
+open PotentialTerm
+open ChargeProfile
+open CodimensionOneConfig
+open Tree Leaf Twig Branch Trunk
+
+/-!
+
+### phenoInsertQ5 on nonPhenoConstrainedCharges is empty
+
+This result is used to help show completeness.
+
+-/
+
+lemma nonPhenoConstrainedCharges_phenoInsertQ5_card_zero_same : ∀ q5 ∈ same.allowedBarFiveCharges,
+    (phenoInsertQ5 (nonPhenoConstrainedCharges same) q5).card = 0 := by
+  decide
+
+lemma nonPhenoConstrainedCharges_phenoInsertQ5_card_zero_nearestNeighbor :
+    ∀ q5 ∈ nearestNeighbor.allowedBarFiveCharges,
+    (phenoInsertQ5 (nonPhenoConstrainedCharges nearestNeighbor) q5).card = 0 := by
+  decide
+
+lemma nonPhenoConstrainedCharges_phenoInsertQ5_card_zero_nextToNearestNeighbor :
+    ∀ q5 ∈ nextToNearestNeighbor.allowedBarFiveCharges,
+    (phenoInsertQ5 (nonPhenoConstrainedCharges nextToNearestNeighbor) (q5)).card = 0 := by
+  decide
+
+lemma nonPhenoConstrainedCharges_phenoInsertQ5_card_zero (I : CodimensionOneConfig) :
+    ∀ q5 ∈ I.allowedBarFiveCharges,
+    (phenoInsertQ5 (nonPhenoConstrainedCharges I) q5).card = 0 :=
+  match I with
+  | same => nonPhenoConstrainedCharges_phenoInsertQ5_card_zero_same
+  | nearestNeighbor => nonPhenoConstrainedCharges_phenoInsertQ5_card_zero_nearestNeighbor
+  | nextToNearestNeighbor =>
+    nonPhenoConstrainedCharges_phenoInsertQ5_card_zero_nextToNearestNeighbor
+
+end Charges
+
+end SU5U1
+
+end FTheory
